EqualProps.thy
@@ -1,0 +1,90 @@
+(*  Title:  HoTT/EqualProps.thy
+    Author: Josh Chen
+    Date:   Jun 2018
+
+Properties of equality.
+*)
+
+theory EqualProps
+  imports
+    HoTT_Methods
+    Equal
+    Prod
+begin
+
+section \<open>Symmetry / Path inverse\<close>
+
+definition inv :: "[Term, Term, Term] \<Rightarrow> Term"  ("(1inv[_,/ _,/ _])")
+  where "inv[A,x,y] \<equiv> \<^bold>\<lambda>p: (x =\<^sub>A y). indEqual[A] (\<lambda>x y _. y =\<^sub>A x) (\<lambda>x. refl(x)) x y p"
+
+lemma inv_type:
+  assumes "p : x =\<^sub>A y"
+  shows "inv[A,x,y]`p : y =\<^sub>A x"
+
+proof
+  show "inv[A,x,y] : (x =\<^sub>A y) \<rightarrow> (y =\<^sub>A x)"
+  proof (unfold inv_def, standard)
+    fix p assume asm: "p : x =\<^sub>A y"
+    show "indEqual[A] (\<lambda>x y _. y =[A] x) refl x y p : y =\<^sub>A x"
+    proof standard+
+      show "x : A" by (wellformed jdgmt: asm)
+      show "y : A" by (wellformed jdgmt: asm)
+    qed (assumption | rule | rule asm)+
+  qed (wellformed jdgmt: assms)
+qed (rule assms)
+      
+
+lemma inv_comp:
+  assumes "a : A"
+  shows "inv[A,a,a]`refl(a) \<equiv> refl(a)"
+
+proof -
+  have "inv[A,a,a]`refl(a) \<equiv> indEqual[A] (\<lambda>x y _. y =\<^sub>A x) (\<lambda>x. refl(x)) a a refl(a)"
+  proof (unfold inv_def, standard)
+    show "refl(a) : a =\<^sub>A a" using assms ..
+
+    fix p assume asm: "p : a =\<^sub>A a"
+    show "indEqual[A] (\<lambda>x y _. y =\<^sub>A x) refl a a p : a =\<^sub>A a"
+    proof standard+
+      show "a : A" by (wellformed jdgmt: asm)
+      then show "a : A" .  \<comment> \<open>The elimination rule requires that both arguments to \<open>indEqual\<close> be shown to have the correct type.\<close>
+    qed (assumption | rule | rule asm)+
+  qed
+
+  also have "indEqual[A] (\<lambda>x y _. y =\<^sub>A x) (\<lambda>x. refl(x)) a a refl(a) \<equiv> refl(a)"
+    by (standard | assumption | rule assms)+
+
+  finally show "inv[A,a,a]`refl(a) \<equiv> refl(a)" .
+qed
+
+section \<open>Transitivity / Path composition\<close>
+
+\<comment> \<open>"Raw" composition function\<close>
+definition compose' :: "Term \<Rightarrow> Term"  ("(1compose''[_])")
+  where "compose'[A] \<equiv>
+    indEqual[A] (\<lambda>x y _. \<Prod>z:A. \<Prod>q: y =\<^sub>A z. x =\<^sub>A z) (indEqual[A](\<lambda>x z _. x =\<^sub>A z) (\<^bold>\<lambda>x:A. refl(x)))"
+
+\<comment> \<open>"Natural" composition function\<close>
+abbreviation compose :: "[Term, Term, Term, Term] \<Rightarrow> Term"  ("(1compose[_,/ _,/ _,/ _])")
+  where "compose[A,x,y,z] \<equiv> \<^bold>\<lambda>p:x =\<^sub>A y. \<^bold>\<lambda>q:y =\<^sub>A z. compose'[A]`x`y`p`z`q"
+
+(**** GOOD CANDIDATE FOR AUTOMATION ****)
+lemma compose_comp:
+  assumes "a : A"
+  shows "compose[A,a,a,a]`refl(a)`refl(a) \<equiv> refl(a)" using assms Equal_intro[OF assms] unfolding compose'_def by simp
+
+text "The above proof is a good candidate for proof automation; in particular we would like the system to be able to automatically find the conditions of the \<open>using\<close> clause in the proof.
+This would likely involve something like:
+  1. Recognizing that there is a function application that can be simplified.
+  2. Noting that the obstruction to applying \<open>Prod_comp\<close> is the requirement that \<open>refl(a) : a =\<^sub>A a\<close>.
+  3. Obtaining such a condition, using the known fact \<open>a : A\<close> and the introduction rule \<open>Equal_intro\<close>."
+
+lemmas Equal_simps [simp] = inv_comp compose_comp
+
+subsubsection \<open>Pretty printing\<close>
+
+abbreviation inv_pretty :: "[Term, Term, Term, Term] \<Rightarrow> Term"  ("(1_\<^sup>-\<^sup>1[_, _, _])" 500)
+  where "p\<^sup>-\<^sup>1[A,x,y] \<equiv> inv[A,x,y]`p"
+
+abbreviation compose_pretty :: "[Term, Term, Term, Term, Term, Term] \<Rightarrow> Term"  ("(1_ \<bullet>[_, _, _, _]/ _)")
+  where "p \<bullet>[A,x,y,z] q \<equiv> compose[A,x,y,z]`p`q"
